wip

code/rocq/elpi_equiv.v
@@ -2,6 +2,7 @@ From mathcomp Require Import all_ssreflect.
 From det Require Import lang elpi_prop elpi.
 From elpi.apps Require Import derive derive.std.
 From HB Require Import structures.
+From det Require Import zify_ssreflect.
 
 Module NurEqiv (U : Unif).
 
@@ -184,7 +185,7 @@ Module NurEqiv (U : Unif).
         have [H|{}HA] := HA _ _ _ _ _ _ _ vA eA YY.
           by rewrite H/= -/SB size_cat map_cat//; auto.
         rewrite-size_cat HA; right => /=.
-        have:= valid_state_valid_ca_help _ _ _ _ YY vA (leqnn _).
+        have:= valid_state_valid_ca_help YY vA (leqnn _).
         move=>/=; case: suffixP; rewrite /=-!andbA; last first.
           move=> _/and3P[]/eqP?; subst => /=.
           rewrite add_ca_deep_empty2/= => H1 H2.
@@ -242,7 +243,7 @@ Module NurEqiv (U : Unif).
         move=>[??]; subst.
         rewrite size_cat addnK drop_size_cat// take_size_cat//.
         rewrite -cat_cons SB/=.
-        have := valid_state_valid_ca_help _ _ _ _ SA vA (leqnn _).
+        have := valid_state_valid_ca_help SA vA (leqnn _).
         rewrite/= suffix_catr?suffix_refl//suffix_catl//-!andbA.
         rewrite size_cat addnK take_size_cat//.
         move=>/and5P[] _ /suffixP/=[w?]; subst.
@@ -372,19 +373,19 @@ Module NurEqiv (U : Unif).
         runb s A s1 B b -> 
           exists x xs, state_to_list A [::] = x :: xs /\ nur s x xs s1 (state_to_list B [::]).
 
-  Lemma expanded_failedT {A B x xs s b1 l} :
+  Lemma expanded_failedT {A B s b1 l} :
     valid_state A -> failed A ->
-    state_to_list A l = x :: xs -> expandedb s A (Failed B) b1 ->
-        state_to_list B l = x :: xs.
+     expandedb s A (Failed B) b1 ->
+        state_to_list A l = state_to_list B l.
   Proof.
     remember (Failed B).
-    move=> +++ H.
-    elim: H B x xs Heqe l => //=; clear.
-    - move=> s A B HA C x xs [<-] vA H1.
+    move=> ++ H.
+    elim: H B  Heqe l => //=; clear.
+    - move=> s A B HA C [<-] vA H1.
       rewrite -(expand_failure_state_to_list_same HA); auto.
-    - move=> s s' r A B b HA HB IH C x xs ? l vA + sA; subst.
+    - move=> s s' r A B b HA HB IH C ? l vA; subst.
       rewrite (expand_not_failed HA notF)//.
-    - move=> s s' r A B b HA HB IH C x xs ? l vA + sA; subst.
+    - move=> s s' r A B b HA HB IH C ? l vA; subst.
       rewrite (expand_not_failed HA notF)//.
   Qed.
 
@@ -423,7 +424,7 @@ Module NurEqiv (U : Unif).
     valid_state A ->
     failed A = false -> expand s1 A = Expanded s2 B -> 
     state_to_list A l = [::] :: xs ->
-    failed B = false /\ s1 = s2.
+    failed B = false /\ s1 = s2 /\ state_to_list B l = [::] :: xs.
   Proof.
     elim: A B s1 s2 l xs => //=.
     - move=> B s1 s2 _ xs _ _ [_<-]//.
@@ -433,7 +434,9 @@ Module NurEqiv (U : Unif).
         rewrite state_to_list_dead//=.
         case SB: state_to_list => [|[] zs]//=+[?]; subst.
         case e: expand => //[s1' B'|s1' B']/=[?<-]/=; rewrite dA; subst.
-          apply: HB vB fB e SB.
+          have:= HB _ _ _ _ _ vB fB e SB.
+          move=>[H1[H2 H3]]; rewrite H1 H3; subst.
+          rewrite (state_to_list_dead dA)//.
         have[x[tl[[]]]]:= (expand_cb_state_to_list1 [::] vB e).
         rewrite SB//.
       set SB := state_to_list B [::].
@@ -441,7 +444,8 @@ Module NurEqiv (U : Unif).
       rewrite sA; case: y sA => //= sA + [?]; subst.
       case e: expand => //=[s1' A'|s1' A'][?<-]/=; subst;
       rewrite (valid_state_dead1 (valid_state_expand vA e)).
-        apply: HA vA fA e sA.
+        have:= HA _ _ _ _ _ vA fA e sA.
+        by move=>[H1[H2 H3]]; rewrite H1 H3//.
       have[x[tl[[]]]]:= (expand_cb_state_to_list1 SB vA e).
       rewrite sA//.
     - move=> A HA B0 _ B HB C s1 s2 l xs /and5P[_ vA _].
@@ -453,7 +457,8 @@ Module NurEqiv (U : Unif).
         have [hd H]:= base_and_state_to_list bB.
         rewrite sA !H/=.
         case: y sA => //; case: hd H => //= H sA [?]; subst.
-        have [->->]:= (HA _ _ _ _ _ vA fA e sA).
+        have [->[->HH]]:= (HA _ _ _ _ _ vA fA e sA).
+        rewrite HH/=map_id.
         rewrite (base_and_empty_top bB (H [::]))/=andbF//.
       have [??] := expand_solved_same e; subst.
       have [sA _]:= expand_solved_success e.
@@ -461,12 +466,12 @@ Module NurEqiv (U : Unif).
       case e1: expand => //[s3 B'][?<-]/=; subst.
       rewrite success_state_to_list//sA/=.
       rewrite (success_failed _ sA)/=.
-      have [H|[hd[H H1]]] := bbAnd_state_to_list bB; rewrite H map_id.
+      have [H|[hd[H H1]]] := bbAnd_state_to_list bB; rewrite H !map_id.
         apply: HB vB fB e1.
       set X:= (make_lB0 _ _).
       have [y[ys sB]]:= failed_state_to_list vB fB (X++l).
       rewrite sB; case: y sB => // sB [?]; subst.
-      apply: HB vB fB e1 sB.
+      by have [->[->->]]:= HB _ _ _ _ _ vB fB e1 sB.
     Qed.
     
   Lemma expand_exp_failedB {s1 s2 A B l ca gs xs}:
@@ -475,6 +480,7 @@ Module NurEqiv (U : Unif).
     state_to_list A l = (cut ca :: gs) :: xs ->
     failed B = false /\ s1 = s2.
   Proof.
+    Search expand state_to_list cut.
     elim: A B s1 s2 l ca gs xs => //=.
     - move=> p[]//=t s1 s2 _ _ [_<-]//.
     - move=> A HA s B HB C s1 s2 l ca gs xs.
@@ -503,7 +509,7 @@ Module NurEqiv (U : Unif).
         rewrite sA !H/=.
         rewrite (base_and_failed bB) andbF orbF.
         case: y sA => [|[|ca1]gs1]//=sA[??]; subst.
-          apply: expand_exp_failed1 vA fA e sA.
+          by have [->[->]]:= expand_exp_failed1 vA fA e sA.
         move=>?; subst; apply: HA vA fA e sA.
       have [??] := expand_solved_same e; subst.
       have [sA _]:= expand_solved_success e.
@@ -519,56 +525,184 @@ Module NurEqiv (U : Unif).
       apply: HB vB fB e1 sB.
   Qed.
 
+  Lemma failed_big_or p s t: failed (big_or p s t).
+  Proof. rewrite/big_or; case: F => //-[]//. Qed.
+
+  Lemma expand_exp_call_failedB {s1 s2 A B l p t gs xs}:
+    valid_state A ->
+    failed A = false -> expand s1 A = Expanded s2 B -> 
+    state_to_list A l = (call p t :: gs) :: xs ->
+    F p t s1 = [::] ->
+    (failed B * (state_to_list B l = xs))%type \/ ((s1 = s2) * ((failed B = false) * (state_to_list B l = (call p t :: gs) :: xs)))%type.
+  Proof.
+    elim: A B s1 s2 l p t gs xs => //=.
+    - move=> p[]//=t C s1 s2 l p1 t1 gs xs _ _ [_<-][??]??; subst.
+      rewrite failed_big_or/big_or=>->; auto.
+    - move=> A HA s B HB C s1 s2 l p t gs xs++++FF.
+      case: ifP => //[dA vB fB|dA /andP[vA bB] fA].
+        rewrite state_to_list_dead//=.
+        case SB: state_to_list => [|[|[p1 t1|] tl] ys]//=+[????]; subst.
+        case e: expand => //[s1' B'|s1' B']/=[?<-]/=; subst; rewrite dA.
+          have [H|H]:= HB _ _ _ _ _ _ _ _ vB fB e SB FF; rewrite !H; auto.
+            left; rewrite state_to_list_dead//=.
+            rewrite -(add_ca_deep_more_less _ 1)//?addn1//.
+            apply: valid_state_valid_ca (valid_state_expand vB e) H.2.
+          by right; rewrite !(state_to_list_dead dA)//.
+        have [w[ws [][]]]:= expand_cb_state_to_list1 [::] vB e.
+        by rewrite SB//.
+      set SB := state_to_list B [::].
+      have [y[ys sA]]:= failed_state_to_list vA fA SB.
+      rewrite sA; case: y sA => //=-[]//=p1 t1 l1 sA + [????]; subst.
+      case e: expand => //=[s1' A'|s1' A'][?<-]/=; subst;
+      rewrite (valid_state_dead1 (valid_state_expand vA e)).
+        have [H|H]:= HA _ _ _ _ _ _ _ _ vA fA e sA FF; rewrite !H-/SB; auto.
+        left; rewrite -(add_ca_deep_more_less _ 1)//?addn1//.
+        rewrite/valid_ca.
+        rewrite valid_ca_split drop_size_cat//.
+        rewrite valid_ca_mn//?size_cat; try lia.
+        have VB := (NurP.bbOr_valid _ _ _ _ _ bB erefl).
+        rewrite VB andbT push_bt_out//cats0.
+        apply: valid_state_valid_ca_help H.2 (valid_state_expand vA e) (leqnn _).    
+      have [w[ws [][]]]:= expand_cb_state_to_list1 SB vA e.
+      by rewrite sA//.
+    - move=> A HA B0 _ B HB C s1 s2 l p t gs xs /and5P[_ vA _]+++++FF.
+      case e: expand => //[s1' A'|s1' A'].
+        have /=fA := expand_not_failed e notF.
+        rewrite (expand_not_solved_not_success e)//fA/=.
+        move=>/eqP->bB _ [?<-]/=; subst.
+        have [y[ys sA]]:= failed_state_to_list vA fA l.
+        have [hd H]:= base_and_state_to_list bB.
+        rewrite sA !H/=.
+        rewrite (base_and_failed bB) andbF orbF.
+        case: y sA => [|[p1 t1|] tl]//=sA[??]; subst.
+          have [H1[H2 H3]]:= (expand_exp_failed1 vA fA e sA); subst.
+          rewrite H1 H3/=map_id H/=; auto.
+        move=>??; subst.
+        have [H1|H1]:= HA _ _ _ _ _ _ _ _ vA fA e sA FF; rewrite !H1/=?H; auto.
+        left; case: ys sA H1 => //=y ys sA H1.
+        rewrite !H/=; rewrite -(add_deep_more_less 1)//?addn1//.
+        have:= valid_state_valid_ca_help H1.2 (valid_state_expand vA e) (leqnn _).
+        move=>/=/andP[_].
+        rewrite -(valid_ca_mn1 1)//addn1//.
+      have [??] := expand_solved_same e; subst.
+      have [sA _]:= expand_solved_success e.
+      rewrite sA/= success_failed//= => vB bB fB.
+      case e1: expand => //[s3 B'][?<-]/=; subst.
+      rewrite (success_failed _ sA)/=sA/=.
+      rewrite success_state_to_list//=.
+      have [H|[hd[H H1]]]:= bbAnd_state_to_list bB; rewrite H map_id.
+        rewrite map_id => Hz.
+        apply: HB vB fB e1 Hz FF.
+      set X := make_lB0 _ _.
+      have [y[ys sB]]:= failed_state_to_list vB fB (X++l).
+      rewrite sB map_id; case: y sB => //-[]//p1 t1 l1 sB []????; subst.
+      have [Hz|Hz]:= HB _ _ _ _ _ _ _ _ vB fB e1 sB FF; rewrite !Hz/=; auto.
+  Qed.
+
+  Lemma zzzzz {s' B C b l p t gs xs}:
+    valid_state B ->
+    failed B = false ->
+    expandedb s' B (Failed C) b ->
+    state_to_list B l = (call p t :: gs) :: xs ->
+    F p t s' = [::] ->
+    state_to_list C l = xs.
+  Proof.
+    remember (Failed C) as F eqn:HF.
+    move=> ++H.
+    elim: H C l p t gs xs HF => //; clear.
+    - move=> s A B HA C l p t gs xs [?] vA.
+      rewrite (expand_failure_failed HA)//.
+    - move=> s s' r A B b HA HB IH C l p t gs xs ? vA fA + FF; subst.
+      have [x[tl[H1 H2]]] := (expand_cb_state_to_list1 l vA HA).
+      rewrite H1//.
+    - move=> s s' r A B b HA HB IH C l p t gs xs ? vA fA HH FF; subst.
+      have [H|[? H]]:= expand_exp_call_failedB vA fA HA HH FF; subst.
+        rewrite-(expanded_failedT (valid_state_expand vA HA) H.1 HB) H//.
+      by have:= IH _ _ _ _ _ _ erefl (valid_state_expand vA HA) H.1 H.2 FF.
+  Qed.
+
+
   Definition is_call l:= match l with call _ _ => true | _ => false end.
 
-  Fixpoint will_call l :=
+  Fixpoint will_call l ca :=
     match l with
     | [::] => None
-    | cut _ :: l => will_call l
-    | call _ _ as c :: _ => Some c
+    | cut ca :: l => will_call l ca
+    | call pr t :: _ => Some (pr,t,ca)
     end.
 
-  Lemma will_call_catr pref w z:
-    will_call w = Some z ->
-      exists z0 : G, will_call (pref ++ w) = Some z0.
+  (* Lemma will_call_catr pref w z:
+    will_call w ca = Some z ->
+      exists z0, will_call (pref ++ w) = Some z0.
   Proof.
     elim: pref w z => //.
       move=> w z ->; by eexists.
     move=> []//=; by eexists.
+  Qed. *)
+
+  Lemma will_call_suff hd l p t ca:
+    all empty_ca hd ->
+    will_call hd l = Some (p, t, ca) ->
+    will_call hd [::] = Some (p, t, [::]).
+  Proof.
+    elim: hd l p t ca => //=-[p t|ca] tl IH.
+      move=> l p1 t1 ca1 /andP[H1 H2] [???]; subst.
+      move=>//.
+    case: ca => //= _ p1 t1 ca1.
+    apply: IH.
   Qed.
 
-  Lemma expanded_failedF {A B x xs s b1 l} :
+  Lemma expanded_failedF {A B C x xs s b1 l y ys} :
     valid_state A -> failed A = false ->
     state_to_list A l = x :: xs -> expandedb s A (Failed B) b1 ->
-        exists z, (will_call x) = Some z.
+          state_to_list C l = y :: ys ->
+        exists p t ca, (will_call x xs) = Some (p,t,ca) /\
+          if F p t s == [::] then y::ys = ca
+          else true.
   Proof.
     remember (Failed B).
     move=> +++ H.
-    elim: H B x xs Heqe l => //=; clear.
-    - move=> s A B HA C x xs _ l _.
+    elim: H B C x xs y ys Heqe l => //=; clear.
+    - move=> s A B HA C D x xs y ys _ l _.
       rewrite (expand_failure_failed HA)//.
-    - move=> s s' r A B b HA HB IH C x xs ? l vA fA sA; subst.
+    - move=> s s' r A B b HA HB IH C D x xs y ys ? l vA fA sA sD; subst.
       have [hd[tl[[+ H2] H3]]]:= expand_cb_state_to_list1 l vA HA.
       rewrite sA => -[??]; subst => /=.
-      apply: IH erefl _ (valid_state_expand vA HA) _ (H2 [::]).
-      apply: expand_cb_failedB vA fA HA.
-    - move=> s s' r A B b HA HB IH C x xs ? l vA fA sA; subst.
-      have vB := (valid_state_expand vA HA).
+      have fB := expand_cb_failedB vA fA HA.
+      have:= IH _ _ _ _ _ _ erefl _ (valid_state_expand vA HA) fB (H2 _) sD.
+      rewrite (expand_cb_same_subst HA). 
+      move=>[p[t [ca[Hs Ht]]]].
+      eexists p, t, [::]; split => //.
+        apply: will_call_suff H3 Hs.
+      move: Ht; case: ifP => ///eqP HH ?; subst.
+      (* this is false: B = hd with empty ca, the first goal in B has no impl,
+         therefore next_alt C = None, but by hyp it is Somw *)
+      admit.
+    - move=> s s' r A B b HA HB IH C D x xs y ys ? l vA fA sA sD; subst.
+      have /= vB := (valid_state_expand vA HA).
+      have /= vC := (valid_state_expanded vB (ex_intro _ _ HB)).
       case: x sA => //.
         move=> sA.
         have sB := state_to_list_hd0 vA sA HA.
-        apply: IH erefl _ vB _ sB.
-        apply: proj1 (expand_exp_failed1 vA fA HA sA).
+        have [fB [? _]] := expand_exp_failed1 vA fA HA sA; subst.
+        apply: IH erefl _ vB fB sB sD.
       move=>[p t|ca] gs H/=.
-        by eexists.
+        do 3 eexists; split => //.
+        case: ifP => ///eqP FF.
+        admit.
       have [fB ?] := expand_exp_failedB vA fA HA H; subst.
       have:= state_to_list_expand vA HA H => -[]H1.
-        apply: IH erefl _ vB fB H1.
-      have /=[y[ys Hy]]:= failed_state_to_list vB fB l.
-      move: H1; rewrite Hy.
+        apply: IH erefl _ vB fB H1 sD.
+      have /=[w[ws Hw]]:= failed_state_to_list vB fB l.
+      move: H1; rewrite Hw.
       move=>[??]; subst.
-      apply: IH erefl _ vB fB Hy.
-  Qed.
+      have:= IH _ _ _ _ _ _ erefl _ (vB) (fB) (Hw) (sD).
+      move=>[p[t[ca[Ha Hb]]]].
+      eexists p, t, _.
+      admit.
+      (*gs fails, therefore execting HB fix y::ys to somthing which a suff for w::l*)  
+      (* everything should go smooth *)
+  Admitted.
 
   Lemma runElpiP: forall A, runElpi A.
   Proof.
@@ -588,17 +722,23 @@ Module NurEqiv (U : Unif).
       rewrite sA.
       have ? := same_subst s s'; subst.
       exists x, xs; split => //.
+      rewrite -(failed_next_alt_some_state_to_list (valid_state_expanded vA (ex_intro _ _ HA)) (expandedb_failed HA) HB)/= in sC'.
       case f: (failed A).
-        have := expanded_failedT vA f sA HA.
-        rewrite (failed_next_alt_some_state_to_list (valid_state_expanded vA (ex_intro _ _ HA)) (expandedb_failed HA) HB).
-        rewrite sC' => -[]??; subst => //.
-      have:= expanded_failedF vA f sA HA.
-      move=>[z].
-      (* admit. *)
-      case: x sA => //-[p t|ca]//=gs sA.  
-        move=>[]?; subst.
-        apply: CallE.
-        
+        move: sA.
+        rewrite (expanded_failedT vA f HA).
+        rewrite sC'.
+        move => -[]??; subst => //.
+      have [p[t[ca[H1 H2]]]]:= expanded_failedF vA f sA HA sC'.
+      elim: x xs H1 H2 {sA} => //-[p1 t1|ca1]/= gs IH xs H1 H2.
+        move: H1 => -[???]; subst.
+        move: H2; case: ifP => /eqP FF?; subst.
+          apply: FailE FF H.
+        move: FF; case FF: F => //[r rs] _. 
+        apply: CallE FF _.
+        rewrite/save_alt.
+        admit.
+      apply: CutE.
+      apply: IH H1 H2.
   Admitted.
   Print Assumptions runElpiP.
 End NurEqiv.
